coq_translation/examples-from-rust-book/error_handling/combinators_map.v
@@ -123,27 +123,27 @@ Module Impl__crate_fmt_Debug_for_Cooked.
   }.
 End Impl__crate_fmt_Debug_for_Cooked.
 
-Definition peel (food : Option) : Option :=
+Definition peel (food : Option Food) : Option Peeled :=
   match food with
   | 'Some.Build_t food => Some (Peeled.Build_t food)
   | None => None
   end.
 
-Definition chop (peeled : Option) : Option :=
+Definition chop (peeled : Option Peeled) : Option Chopped :=
   match peeled with
   | 'Some.Build_t 'Peeled.Build_t food => Some (Chopped.Build_t food)
   | None => None
   end.
 
-Definition cook (chopped : Option) : Option :=
+Definition cook (chopped : Option Chopped) : Option Cooked :=
   chopped.["map"] (fun 'Chopped.Build_t food => Cooked.Build_t food).
 
-Definition process (food : Option) : Option :=
+Definition process (food : Option Food) : Option Cooked :=
   ((food.["map"] (fun f => Peeled.Build_t f)).["map"]
       (fun 'Peeled.Build_t f => Chopped.Build_t f)).["map"]
     (fun 'Chopped.Build_t f => Cooked.Build_t f).
 
-Definition eat (food : Option) : unit :=
+Definition eat (food : Option Cooked) : unit :=
   match food with
   | 'Some.Build_t food =>
     _crate.io._print
