coq_translation/examples-from-rust-book/generics/generics_new_type_idiom_as_base_type.v
@@ -15,5 +15,5 @@ Definition Years := Years.t.
 Definition main (_ : unit) : unit :=
   let years := Years.Build_t 42 in
   let years_as_primitive_1 := years .[ 0 ] in
-  let 'Years.Build_t years_as_primitive_2 := years in
+  let ''Years.Build_t years_as_primitive_2 := years in
   tt.
